src/semantics/Event.v
@@ -1,0 +1,179 @@
+From sflib Require Import sflib.
+From Fairness Require Export ITreeLib Any Optics.
+From Coq Require Import Classes.RelationClasses Program.
+From Coq Require Export Strings.String.
+
+Set Implicit Arguments.
+
+Module Flag.
+
+  Variant t: Type :=
+  | fail
+  | emp
+  | success
+  .
+
+  Definition le: t -> t -> Prop :=
+    fun f0 f1 =>
+      match f0, f1 with
+      | fail, _ => True
+      | _, fail => False
+      | emp, _ => True
+      | _, emp => False
+      | success, _ => True
+      end.
+
+  Global Program Instance le_PreOrder: PreOrder le.
+  Next Obligation.
+    ii. destruct x; ss.
+  Qed.
+  Next Obligation.
+    ii. destruct x, y, z; ss.
+  Qed.
+
+End Flag.
+
+Section IDENT.
+
+  Definition ID := Type.
+
+  Definition id_prod (A B: ID): ID := (prod A B).
+  Definition id_sum (A B: ID): ID := (sum A B).
+
+  (* Class ID : Type := mk_id { id: Type }. *)
+
+  (* Definition id_prod (A B: ID): ID := mk_id (prod A.(id) B.(id)). *)
+  (* Definition id_sum (A B: ID): ID := mk_id (sum A.(id) B.(id)). *)
+
+End IDENT.
+
+Section EVENT.
+
+  (* Context {Ident: ID}. *)
+
+  Definition fmap (id: ID) := id -> Flag.t.
+
+  Variant eventE {id: ID}: Type -> Type :=
+    | Choose (X: Type): eventE X
+    | Fair (m: @fmap id): eventE unit
+    | Observe (fn: nat) (args: list nat): eventE nat
+    | Undefined: eventE void
+  .
+
+  Definition UB {id: ID} {E} `{@eventE id -< E} {R}:
+    itree E R :=
+    f <- trigger Undefined;;
+    match (f: void) with end.
+
+  Definition unwrap {id: ID} {E} `{@eventE id -< E} {R}
+             (r: option R): itree E R :=
+    match r with
+    | Some r => Ret r
+    | None => UB
+    end.
+
+End EVENT.
+
+Notation fname := string (only parsing).
+Notation thread_id := nat (only parsing).
+
+Section EVENTS.
+
+  Variant cE: Type -> Type :=
+  | Yield: cE unit
+  | GetTid: cE thread_id
+  (* | Spawn (fn: fname) (args: list Val): cE unit *)
+  .
+
+  (* sE is just state monad *)
+  Variant sE (S : Type) (X : Type) : Type :=
+  | Rmw (rmw : S -> S * X) : sE S X
+  .
+
+  Variant callE: Type -> Type :=
+  | Call (fn: fname) (arg: Any.t): callE Any.t
+  .
+
+  Definition Get {S} {X} (p : S -> X) : sE S X := Rmw (fun x => (x, p x)).
+  Definition Put {S} (x' : S) : sE S () := Rmw (fun x => (x', tt)).
+  Definition Modify {S} (f : S -> S) : sE S () := Rmw (fun x => (f x, tt)).
+
+  Lemma get_rmw {S X} (p : S -> X) : Get p = Rmw (fun x => (x, p x)).
+  Proof. reflexivity. Qed.
+
+  Lemma put_rmw {S} (x' : S) : Put x' = Rmw (fun x => (x', tt)).
+  Proof. reflexivity. Qed.
+
+  Lemma modify_rmw {S} (f : S -> S) : Modify f = Rmw (fun x => (f x, tt)).
+  Proof. reflexivity. Qed.
+
+End EVENTS.
+
+Global Opaque Get.
+Global Opaque Put.
+Global Opaque Modify.
+
+Notation programE ident State :=
+  ((((@eventE ident) +' cE) +' callE) +' sE State).
+
+Section LENS.
+
+  Variable S: Type.
+  Variable V: Type.
+
+  Variable l : Lens.t S V.
+
+  Definition lens_rmw X : (V -> V * X) -> (S -> S * X) :=
+    fun rmw s =>
+      (Lens.set l (fst (rmw (Lens.view l s))) s, snd (rmw (Lens.view l s))).
+
+  Definition map_lens X (se : sE V X) : sE S X :=
+    match se with
+    | Rmw rmw => Rmw (lens_rmw rmw)
+    end.
+
+End LENS.
+
+Section PRISM.
+
+  Variable S : Type.
+  Variable A : Type.
+
+  Variable p : Prism.t S A.
+
+  Definition prism_fmap : fmap A -> fmap S :=
+    fun fm i =>
+      match Prism.preview p i with
+      | None => Flag.emp
+      | Some j => fm j
+      end.
+
+  Definition map_prism X : @eventE A X -> @eventE S X :=
+    fun e =>
+      match e with
+      | Choose X => Choose X
+      | Fair fm => Fair (prism_fmap fm)
+      | Observe fn args => Observe fn args
+      | Undefined => Undefined
+      end.
+
+End PRISM.
+
+Section PROGRAM_EVENT.
+
+  Variable ident ident' : Type.
+  Variable state state' : Type.
+
+  Variable p : Prism.t ident' ident.
+  Variable l : Lens.t state' state.
+
+  Definition plmap X : programE ident state X -> programE ident' state' X.
+  Proof.
+    intro e. destruct e as [[[e|e]|e]|e].
+    - exact ((((map_prism p e)|)|)|)%sum.
+    - exact (((|e)|)|)%sum.
+    - exact ((|e)|)%sum.
+    - exact (|map_lens l e)%sum.
+  Defined.
+
+End PROGRAM_EVENT.
