src/simulation/ModAdequacy.v
@@ -69,9 +69,9 @@ Section LADEQ.
               (<<OSWF: (forall tid', Th.In tid' ths_src -> Th.In tid' os) /\ (Th.find tid os = None)>>) /\
               (<<LSIM:
                 forall im_tgt0
-                  (FAIR: fair_update im_tgt im_tgt0 (sum_fmap_l (tids_fmap tid (NatSet.add tid (key_set ths_tgt))))),
+                  (FAIR: fair_update im_tgt im_tgt0 (prism_fmap inlp (tids_fmap tid (NatSet.add tid (key_set ths_tgt))))),
                 exists im_src0,
-                  (fair_update im_src im_src0 (sum_fmap_l (tids_fmap tid (NatSet.add tid (key_set ths_src))))) /\
+                  (fair_update im_src im_src0 (prism_fmap inlp (tids_fmap tid (NatSet.add tid (key_set ths_src))))) /\
                     (ModSimStutter.lsim (wf_stt) I tid (local_RR I RR tid)
                           ps pt (sum_of_resources rs_ctx) (o, src) tgt
                           (NatSet.add tid (key_set ths_src),
@@ -167,7 +167,7 @@ Section LADEQ.
       rewrite <- nm_find_some_rm_add_eq; auto. eapply nm_elements_cons_find_some; eauto.
     }
     { r_wf IND0. }
-    { instantiate (2:=im_tgt). instantiate (1:=im_tgt). clear. ii. unfold sum_fmap_l. des_ifs. }
+    { instantiate (2:=im_tgt). instantiate (1:=im_tgt). clear. ii. unfold prism_fmap; ss. des_ifs. }
     i; des.
     assert (WFPAIR: nm_wf_pair (NatMap.remove (elt:=thread _ident_src (sE state_src) R0) tid1 ths_src) rs_local).
     { hexploit list_forall4_implies_forall2_3. eauto.
