src/simulation/ModSimYOrd.v
@@ -132,7 +132,7 @@ Section PRIMIVIESIM.
       f_src f_tgt r_ctx os ot
       ths im_src im_tgt0 st_src st_tgt
       f itr_src ktr_tgt
-      (LSIM: forall im_tgt1 (FAIR: fair_update im_tgt0 im_tgt1 (sum_fmap_r f)),
+      (LSIM: forall im_tgt1 (FAIR: fair_update im_tgt0 im_tgt1 (prism_fmap inrp f)),
           (<<LSIM: _lsim _ _ RR f_src true r_ctx (os, itr_src) (ot, ktr_tgt tt) (ths, im_src, im_tgt1, st_src, st_tgt)>>))
     :
     __lsim tid lsim _lsim RR f_src f_tgt r_ctx (os, itr_src) (ot, trigger (Fair f) >>= ktr_tgt) (ths, im_src, im_tgt0, st_src, st_tgt)
@@ -172,7 +172,7 @@ Section PRIMIVIESIM.
                (INV: I (ths1, im_src1, im_tgt1, st_src1, st_tgt1) r_shared1)
                (VALID: URA.wf (r_shared1 ⋅ r_own ⋅ r_ctx1))
                im_tgt2
-               (TGT: fair_update im_tgt1 im_tgt2 (sum_fmap_l (tids_fmap tid ths1))),
+               (TGT: fair_update im_tgt1 im_tgt2 (prism_fmap inlp (tids_fmap tid ths1))),
         exists os1 ot1,
           (<<LSIM: _lsim _ _ RR f_src true r_ctx1 (os1, trigger (Yield) >>= ktr_src) (ot1, ktr_tgt tt) (ths1, im_src1, im_tgt2, st_src1, st_tgt1)>>) /\
             (<<LT: (wf_stt R0 R1).(lt) ot1 ot>>))
@@ -189,7 +189,7 @@ Section PRIMIVIESIM.
                (INV: I (ths1, im_src1, im_tgt1, st_src1, st_tgt1) r_shared1)
                (VALID: URA.wf (r_shared1 ⋅ r_own ⋅ r_ctx1))
                im_tgt2
-               (TGT: fair_update im_tgt1 im_tgt2 (sum_fmap_l (tids_fmap tid ths1))),
+               (TGT: fair_update im_tgt1 im_tgt2 (prism_fmap inlp (tids_fmap tid ths1))),
         exists os1 ot1,
           (<<LSIM: lsim _ _ RR true true r_ctx1 (os1, ktr_src tt) (ot1, ktr_tgt tt) (ths1, im_src1, im_tgt2, st_src1, st_tgt1)>>))
     :
@@ -731,14 +731,14 @@ Section PRIMIVIESIM.
       (THS: TIdSet.add_new tid ths0 ths1)
       (VALID: URA.wf (r_shared0 ⋅ r_ctx0)),
     forall im_tgt0'
-      (UPD: fair_update im_tgt0 im_tgt0' (sum_fmap_l (fun t => if (tid_dec t tid) then Flag.success else Flag.emp))),
+      (UPD: fair_update im_tgt0 im_tgt0' (prism_fmap inlp (fun t => if (tid_dec t tid) then Flag.success else Flag.emp))),
     exists r_shared1 r_own os ot,
       (<<INV: I (ths1, im_src0, im_tgt0', st_src0, st_tgt0) r_shared1>>) /\
         (<<VALID: URA.wf (r_shared1 ⋅ r_own ⋅ r_ctx0)>>) /\
         (forall ths im_src1 im_tgt1 st_src st_tgt r_shared2 r_ctx2
            (INV: I (ths, im_src1, im_tgt1, st_src, st_tgt) r_shared2)
            (VALID: URA.wf (r_shared2 ⋅ r_own ⋅ r_ctx2)),
-          forall im_tgt2 (TGT: fair_update im_tgt1 im_tgt2 (sum_fmap_l (tids_fmap tid ths))),
+          forall im_tgt2 (TGT: fair_update im_tgt1 im_tgt2 (prism_fmap inlp (tids_fmap tid ths))),
             (<<LSIM: forall fs ft,
                 lsim
                   tid
@@ -756,7 +756,7 @@ Section PRIMIVIESIM.
     forall ths im_src im_tgt st_src st_tgt r_shared r_ctx
            (INV: I (ths, im_src, im_tgt, st_src, st_tgt) r_shared)
            (VALID: URA.wf (r_shared ⋅ r_own ⋅ r_ctx)),
-    forall im_tgt1 (FAIR: fair_update im_tgt im_tgt1 (sum_fmap_l (tids_fmap tid ths))),
+    forall im_tgt1 (FAIR: fair_update im_tgt im_tgt1 (prism_fmap inlp (tids_fmap tid ths))),
     forall fs ft,
       lsim
         tid
